src/typechecker/FStar.TypeChecker.Quals.fst
@@ -1,0 +1,229 @@
+(*
+   Copyright 2008-2024 Nikhil Swamy and Microsoft Research
+
+   Licensed under the Apache License, Version 2.0 (the "License");
+   you may not use this file except in compliance with the License.
+   You may obtain a copy of the License at
+
+       http://www.apache.org/licenses/LICENSE-2.0
+
+   Unless required by applicable law or agreed to in writing, software
+   distributed under the License is distributed on an "AS IS" BASIS,
+   WITHOUT WARRANTIES OR CONDITIONS OF ANY KIND, either express or implied.
+   See the License for the specific language governing permissions and
+   limitations under the License.
+*)
+
+module FStar.TypeChecker.Quals
+open FStar
+open FStar.Compiler
+open FStar.Compiler.Effect
+open FStar.Errors
+open FStar.Errors.Msg
+open FStar.Pprint
+open FStar.Syntax.Syntax
+open FStar.Ident
+open FStar.Syntax
+open FStar.Class.Show
+open FStar.Class.PP
+
+module SS = FStar.Syntax.Subst
+module S  = FStar.Syntax.Syntax
+module BU = FStar.Compiler.Util
+module U  = FStar.Syntax.Util
+module N  = FStar.TypeChecker.Normalize
+module C  = FStar.Parser.Const
+
+let check_sigelt_quals_pre (env:FStar.TypeChecker.Env.env) se =
+    let visibility = function Private -> true | _ -> false in
+    let reducibility = function
+        | Irreducible
+        | Unfold_for_unification_and_vcgen | Visible_default
+        | Inline_for_extraction -> true
+        | _ -> false in
+    let assumption = function Assumption | New -> true | _ -> false in
+    let reification = function Reifiable | Reflectable _ -> true | _ -> false in
+    let inferred = function
+      | Discriminator _
+      | Projector _
+      | RecordType _
+      | RecordConstructor _
+      | ExceptionConstructor
+      | HasMaskedEffect
+      | Effect -> true
+      | _ -> false in
+    let has_eq = function Noeq | Unopteq -> true | _ -> false in
+    let quals_combo_ok quals q =
+        match q with
+        | Assumption ->
+          quals
+          |> List.for_all (fun x -> x=q
+                              || x=Logic
+                              || inferred x
+                              || visibility x
+                              || assumption x
+                              || (env.is_iface && x=Inline_for_extraction)
+                              || x=NoExtract)
+
+        | New -> //no definition provided
+          quals
+          |> List.for_all (fun x -> x=q || inferred x || visibility x || assumption x)
+
+        | Inline_for_extraction ->
+          quals |> List.for_all (fun x -> x=q || x=Logic || visibility x || reducibility x
+                                              || reification x || inferred x || has_eq x
+                                              || (env.is_iface && x=Assumption)
+                                              || x=NoExtract)
+
+        | Unfold_for_unification_and_vcgen
+        | Visible_default
+        | Irreducible
+        | Noeq
+        | Unopteq ->
+          quals
+          |> List.for_all (fun x -> x=q || x=Logic || x=Inline_for_extraction || x=NoExtract || has_eq x || inferred x || visibility x || reification x)
+
+        | TotalEffect ->
+          quals
+          |> List.for_all (fun x -> x=q || inferred x || visibility x || reification x)
+
+        | Logic ->
+          quals
+          |> List.for_all (fun x -> x=q || x=Assumption || inferred x || visibility x || reducibility x)
+
+        | Reifiable
+        | Reflectable _ ->
+          quals
+          |> List.for_all (fun x -> reification x || inferred x || visibility x || x=TotalEffect || x=Visible_default)
+
+        | Private ->
+          true //only about visibility; always legal in combination with others
+
+        | _ -> //inferred
+          true
+    in
+    let check_no_subtyping_attribute se =
+      if U.has_attribute se.sigattrs C.no_subtping_attr_lid &&
+         (match se.sigel with
+          | Sig_let _ -> false
+          | _ -> true)
+      then raise_error_doc
+             (Errors.Fatal_InconsistentQualifierAnnotation, [
+              text "Illegal attribute: the `no_subtyping` attribute is allowed only on let-bindings."])
+             se.sigrng in
+    check_no_subtyping_attribute se;
+    let quals = U.quals_of_sigelt se |> List.filter (fun x -> not (x = Logic)) in  //drop logic since it is deprecated
+    if quals |> BU.for_some (function OnlyName -> true | _ -> false) |> not
+    then
+      let r = U.range_of_sigelt se in
+      let no_dup_quals = BU.remove_dups (fun x y -> x=y) quals in
+      let err' msg =
+          raise_error (Errors.Fatal_QulifierListNotPermitted, (BU.format2
+                          "The qualifier list \"[%s]\" is not permissible for this element%s"
+                          (Print.quals_to_string quals) msg)) r in
+      let err msg = err' (": " ^ msg) in
+      let err' () = err' "" in
+      if List.length quals <> List.length no_dup_quals
+      then err "duplicate qualifiers";
+      if not (quals |> List.for_all (quals_combo_ok quals))
+      then err "ill-formed combination";
+      match se.sigel with
+      | Sig_let {lbs=(is_rec, _)} -> //let rec
+        if is_rec && quals |> List.contains Unfold_for_unification_and_vcgen
+        then err "recursive definitions cannot be marked inline";
+        if quals |> BU.for_some (fun x -> assumption x || has_eq x)
+        then err "definitions cannot be assumed or marked with equality qualifiers"
+      | Sig_bundle _ ->
+        if not (quals |> BU.for_all (fun x ->
+              x=Inline_for_extraction
+              || x=NoExtract
+              || inferred x
+              || visibility x
+              || has_eq x))
+        then err' ();
+        if quals |> List.existsb (function Unopteq -> true | _ -> false) &&
+           U.has_attribute se.sigattrs FStar.Parser.Const.erasable_attr
+        then err "unopteq is not allowed on an erasable inductives since they don't have decidable equality"
+      | Sig_declare_typ _ ->
+        if quals |> BU.for_some has_eq
+        then err' ()
+      | Sig_assume _ ->
+        if not (quals |> BU.for_all (fun x -> visibility x || x=Assumption || x=InternalAssumption))
+        then err' ()
+      | Sig_new_effect _ ->
+        if not (quals |> BU.for_all (fun x ->
+              x=TotalEffect
+              || inferred x
+              || visibility x
+              || reification x))
+        then err' ()
+      | Sig_effect_abbrev _ ->
+        if not (quals |> BU.for_all (fun x -> inferred x || visibility x))
+        then err' ()
+      | _ -> ()
+
+let check_erasable env quals r se =
+  let lids = U.lids_of_sigelt se in
+  let val_exists =
+    lids |> BU.for_some (fun l -> Option.isSome (Env.try_lookup_val_decl env l))
+  in
+  let val_has_erasable_attr =
+    lids |> BU.for_some (fun l ->
+      let attrs_opt = Env.lookup_attrs_of_lid env l in
+      Option.isSome attrs_opt
+      && U.has_attribute (Option.get attrs_opt) FStar.Parser.Const.erasable_attr)
+  in
+  let se_has_erasable_attr = U.has_attribute se.sigattrs FStar.Parser.Const.erasable_attr in
+  if ((val_exists && val_has_erasable_attr) && not se_has_erasable_attr)
+  then raise_error_doc (Errors.Fatal_QulifierListNotPermitted, [
+           text "Mismatch of attributes between declaration and definition.";
+           text "Declaration is marked `erasable` but the definition is not.";
+         ]) r;
+  if ((val_exists && not val_has_erasable_attr) && se_has_erasable_attr)
+  then raise_error_doc (Errors.Fatal_QulifierListNotPermitted, [
+           text "Mismatch of attributes between declaration and definition.";
+           text "Definition is marked `erasable` but the declaration is not.";
+         ]) r;
+  if se_has_erasable_attr
+  then begin
+    match se.sigel with
+    | Sig_bundle _ ->
+      if not (quals |> BU.for_some (function Noeq -> true | _ -> false))
+      then raise_error_doc (Errors.Fatal_QulifierListNotPermitted, [
+              text "Incompatible attributes and qualifiers: \
+               erasable types do not support decidable equality and must be marked `noeq`."
+             ]) r
+    | Sig_declare_typ _ ->
+      ()
+    | Sig_fail _ ->
+      () (* just ignore it, the member ses have the attribute too *)
+
+    | Sig_let {lbs=(false, [lb])} ->
+      let _, body, _ = U.abs_formals lb.lbdef in
+      if not (N.non_info_norm env body)
+      then raise_error_doc
+             (Errors.Fatal_QulifierListNotPermitted, [
+                  text "Illegal attribute: \
+                   the `erasable` attribute is only permitted on inductive type definitions \
+                   and abbreviations for non-informative types.";
+                  text "The term" ^/^ pp body ^/^ text "is considered informative.";
+             ]) body.pos
+
+    | Sig_new_effect ({mname=eff_name}) ->  //AR: allow erasable on total effects
+      if not (List.contains TotalEffect quals)
+      then raise_error_doc (Errors.Fatal_QulifierListNotPermitted, [
+               text "Effect" ^/^ pp eff_name ^/^ text "is marked erasable but only total effects are allowed to be erasable."
+             ]) r
+
+    | _ ->
+      raise_error_doc (Errors.Fatal_QulifierListNotPermitted, [
+          text "Illegal attribute: \
+          the `erasable` attribute is only permitted on inductive type definitions \
+          and abbreviations for non-informative types.";
+        ]) r
+  end
+
+let check_sigelt_quals_post env se =
+  let quals = se.sigquals in
+  let r = se.sigrng in
+  check_erasable env quals r se
