src/typechecker/FStar.TypeChecker.Quals.fsti
@@ -1,0 +1,36 @@
+(*
+   Copyright 2008-2024 Nikhil Swamy and Microsoft Research
+
+   Licensed under the Apache License, Version 2.0 (the "License");
+   you may not use this file except in compliance with the License.
+   You may obtain a copy of the License at
+
+       http://www.apache.org/licenses/LICENSE-2.0
+
+   Unless required by applicable law or agreed to in writing, software
+   distributed under the License is distributed on an "AS IS" BASIS,
+   WITHOUT WARRANTIES OR CONDITIONS OF ANY KIND, either express or implied.
+   See the License for the specific language governing permissions and
+   limitations under the License.
+*)
+
+module FStar.TypeChecker.Quals
+
+open FStar
+open FStar.Compiler
+open FStar.Syntax.Syntax
+open FStar.TypeChecker.Env
+  
+(*
+Checking qualifiers **and attributes**. This is split in two functions,
+_pre and _post, as some qualifier/attributes must be checked before the function
+is typechecked (or at least it's better/faster to do so) and some can only be checked
+after the function is typechecked.
+
+Currently, the only thing that must be checked after the function is typechecked
+is the "erasable" attribute, which can only be checked when the body of the definition
+is fully elaborated. See #3252.
+*)
+
+val check_sigelt_quals_pre  : env -> sigelt -> unit
+val check_sigelt_quals_post : env -> sigelt -> unit
